backends/hol4/testHashmapScript.sml
@@ -43,7 +43,7 @@ Theorem nth_mut_fwd_spec:
     case nth_mut_fwd ls i of
     | Return x => x = index (u32_to_int i) (list_t_v ls)
     | Fail _ => F
-    | Loop => F
+    | Diverge => F
 Proof
   Induct_on ‘ls’ >> rw [list_t_v_def, len_def] >~ [‘ListNil’]
   >-(massage >> int_tac) >>
@@ -51,6 +51,8 @@ Proof
   fs [index_eq] >>
   progress >> progress
 QED
+
+val _ = register_spec_thm nth_mut_fwd_spec
 
 val _ = new_constant ("insert", “: u32 -> 't -> (u32 # 't) list_t -> (u32 # 't) list_t result”)
 val insert_def = new_axiom ("insert_def", “
@@ -71,10 +73,8 @@ val insert_def = new_axiom ("insert_def", “
 val distinct_keys_def = Define ‘
   distinct_keys (ls : (u32 # 't) list) =
     !i j.
-      0 < i ⇒ i < len ls ==>
-      0 < j ⇒ j < len ls ==>
-      FST (index i ls) = FST (index j ls) ⇒
-      i = j
+      0 ≤ i ⇒ i < j ⇒ j < len ls ⇒
+      FST (index i ls) ≠ FST (index j ls)
 ’
 
 val lookup_raw_def = Define ‘
@@ -87,6 +87,178 @@ val lookup_def = Define ‘
   lookup key ls = lookup_raw key (list_t_v ls)
 ’
 
+(* Lemma about ‘insert’, without the invariant *)
+Theorem insert_lem_aux:
+  !ls key value.
+    (* The keys are pairwise distinct *)
+    case insert key value ls of
+    | Return ls1 =>
+      (* We updated the binding *)
+      lookup key ls1 = SOME value /\
+      (* The other bindings are left unchanged *)
+      (!k. k <> key ==> lookup k ls = lookup k ls1)
+    | Fail _ => F
+    | Diverge => F
+Proof
+  Induct_on ‘ls’ >> rw [list_t_v_def] >~ [‘ListNil’] >>
+  pure_once_rewrite_tac [insert_def] >> rw []
+  >- (rw [lookup_def, lookup_raw_def, list_t_v_def])
+  >- (rw [lookup_def, lookup_raw_def, list_t_v_def]) >>
+  case_tac >> rw []
+  >- (rw [lookup_def, lookup_raw_def, list_t_v_def])
+  >- (rw [lookup_def, lookup_raw_def, list_t_v_def]) >>
+  progress >>
+  fs [lookup_def, lookup_raw_def, list_t_v_def]
+QED
+
+Theorem distinct_keys_cons:
+  ∀ k v ls.
+  (∀ i. 0 ≤ i ⇒ i < len ls ⇒ FST (index i ls) ≠ k) ⇒
+  distinct_keys ls ⇒
+  distinct_keys ((k,v) :: ls)
+Proof
+  rw [] >>
+  rw [distinct_keys_def] >>
+  Cases_on ‘i = 0’ >> fs []
+  >-(
+    (* Use the first hypothesis *)
+    fs [index_eq] >>
+    last_x_assum (qspecl_assume [‘j - 1’]) >>
+    sg ‘0 ≤ j - 1’ >- int_tac >>
+    fs [len_def] >>
+    sg ‘j - 1 < len ls’ >- int_tac >>
+    fs []
+  ) >>
+  (* Use the second hypothesis *)
+  sg ‘0 < i’ >- int_tac >>
+  sg ‘0 < j’ >- int_tac >>
+  fs [distinct_keys_def, index_eq, len_def] >>
+  first_x_assum (qspecl_assume [‘i - 1’, ‘j - 1’]) >>
+  sg ‘0 ≤ i - 1 ∧ i - 1 < j - 1 ∧ j - 1 < len ls’ >- int_tac >>
+  fs []
+QED
+
+Theorem distinct_keys_tail:
+  ∀ k v ls.
+  distinct_keys ((k,v) :: ls) ⇒
+  distinct_keys ls
+Proof
+  rw [distinct_keys_def] >>
+  last_x_assum (qspecl_assume [‘i + 1’, ‘j + 1’]) >>
+  fs [len_def] >>
+  sg ‘0 ≤ i + 1 ∧ i + 1 < j + 1 ∧ j + 1 < 1 + len ls’ >- int_tac >> fs [] >>
+  sg ‘0 < i + 1 ∧ 0 < j + 1’ >- int_tac >> fs [index_eq] >>
+  sg ‘i + 1 - 1 = i ∧ j + 1 - 1 = j’ >- int_tac >> fs []
+QED
+
+Theorem insert_index_neq:
+  ∀ q k v ls0 ls1 i.
+  (∀ j. 0 ≤ j ∧ j < len (list_t_v ls0) ⇒ q ≠ FST (index j (list_t_v ls0))) ⇒
+  q ≠ k ⇒
+  insert k v ls0 = Return ls1 ⇒
+  0 ≤ i ⇒
+  i < len (list_t_v ls1) ⇒
+  FST (index i (list_t_v ls1)) ≠ q
+Proof
+  ntac 3 strip_tac >>
+  Induct_on ‘ls0’ >> rw [] >~ [‘ListNil’]
+  >-(
+    fs [insert_def] >>
+    sg ‘ls1 = ListCons (k,v) ListNil’ >- fs [] >> fs [list_t_v_def, len_def] >>
+    sg ‘i = 0’ >- int_tac >> fs [index_eq]) >>
+  Cases_on ‘t’ >>
+  Cases_on ‘i = 0’ >> fs []
+  >-(
+    qpat_x_assum ‘insert _ _ _ = _’ mp_tac >>
+    simp [MK_BOUNDED insert_def 1, bind_def] >>
+    Cases_on ‘q' = k’ >> rw []
+    >- (fs [list_t_v_def, index_eq]) >>
+    Cases_on ‘insert k v ls0’ >> fs [] >>
+    (* TODO: would be good to have a tactic which inverts equalities of the
+       shape ‘ListCons (q',r) a = ls1’ *)
+    sg ‘ls1 = ListCons (q',r) a’ >- fs [] >> fs [list_t_v_def, index_eq] >>
+    first_x_assum (qspec_assume ‘0’) >>
+    fs [len_def] >>
+    strip_tac >>
+    qspec_assume ‘list_t_v ls0’ len_pos >>
+    sg ‘0 < 1 + len (list_t_v ls0)’ >- int_tac >>
+    fs []) >>
+  qpat_x_assum ‘insert _ _ _ = _’ mp_tac >>
+  simp [MK_BOUNDED insert_def 1, bind_def] >>
+  Cases_on ‘q' = k’ >> rw []
+  >-(
+    fs [list_t_v_def, index_eq, len_def] >>
+    first_x_assum (qspec_assume ‘i’) >> rfs []) >>
+  Cases_on ‘insert k v ls0’ >> fs [] >>
+  sg ‘ls1 = ListCons (q',r) a’ >- fs [] >> fs [list_t_v_def, index_eq] >>
+  last_x_assum (qspec_assume ‘i - 1’) >>
+  fs [len_def] >>
+  sg ‘0 ≤ i - 1 ∧ i - 1 < len (list_t_v a)’ >- int_tac >> fs [] >>
+  first_x_assum irule >>
+  rw [] >>
+  last_x_assum (qspec_assume ‘j + 1’) >>
+  rfs [] >>
+  sg ‘j + 1 < 1 + len (list_t_v ls0) ∧ j + 1 − 1 = j ∧ j + 1 ≠ 0’ >- int_tac >> fs []
+QED
+
+Theorem distinct_keys_insert_index_neq:
+  ∀ k v q r ls0 ls1 i.
+  distinct_keys ((q,r)::list_t_v ls0) ⇒
+  q ≠ k ⇒
+  insert k v ls0 = Return ls1 ⇒
+  0 ≤ i ⇒
+  i < len (list_t_v ls1) ⇒
+  FST (index i (list_t_v ls1)) ≠ q
+Proof
+  rw [] >>
+  (* Use the first assumption to prove the following assertion *)
+  sg ‘∀ j. 0 ≤ j ∧ j < len (list_t_v ls0) ⇒ q ≠ FST (index j (list_t_v ls0))’
+  >-(
+    strip_tac >>
+    fs [distinct_keys_def] >>
+    last_x_assum (qspecl_assume [‘0’, ‘j + 1’]) >>
+    fs [index_eq] >>
+    sg ‘j + 1 - 1 = j’ >- int_tac >> fs [len_def] >>
+    rw []>>
+    first_x_assum irule >> int_tac) >>
+  qspecl_assume [‘q’, ‘k’, ‘v’, ‘ls0’, ‘ls1’, ‘i’] insert_index_neq >>
+  fs []
+QED
+
+Theorem distinct_keys_insert:
+  ∀ k v ls0 ls1.
+  distinct_keys (list_t_v ls0) ⇒
+  insert k v ls0 = Return ls1 ⇒
+  distinct_keys (list_t_v ls1)
+Proof
+  Induct_on ‘ls0’ >~ [‘ListNil’]
+  >-(
+    rw [distinct_keys_def, list_t_v_def, insert_def] >>
+    fs [list_t_v_def, len_def] >>
+    int_tac) >>  
+  Cases >>
+  pure_once_rewrite_tac [insert_def] >> fs[] >>
+  rw [] >> fs []
+  >-(
+    (* k = q *)
+    last_x_assum ignore_tac >>
+    fs [distinct_keys_def] >>
+    rw [] >>
+    last_x_assum (qspecl_assume [‘i’, ‘j’]) >>
+    rfs [list_t_v_def, len_def] >>
+    sg ‘0 < j’ >- int_tac >>
+    Cases_on ‘i = 0’ >> fs [index_eq] >>
+    sg ‘0 < i’ >- int_tac >> fs []) >>
+  (* k ≠ q: recursion *)
+  Cases_on ‘insert k v ls0’ >> fs [bind_def] >>
+  last_x_assum (qspecl_assume [‘k’, ‘v’, ‘a’]) >>
+  rfs [] >>
+  sg ‘ls1 = ListCons (q,r) a’ >- fs [] >> fs [list_t_v_def] >>
+  imp_res_tac distinct_keys_tail >> fs [] >>
+  irule distinct_keys_cons >> rw [] >>
+  metis_tac [distinct_keys_insert_index_neq]
+QED  
+
 Theorem insert_lem:
   !ls key value.
     (* The keys are pairwise distinct *)
@@ -96,28 +268,16 @@ Theorem insert_lem:
       (* We updated the binding *)
       lookup key ls1 = SOME value /\
       (* The other bindings are left unchanged *)
-      (!k. k <> key ==> lookup k ls = lookup k ls1)
-      (* TODO: invariant *)
+      (!k. k <> key ==> lookup k ls = lookup k ls1) ∧
+      (* The keys are still pairwise disjoint *)
+      distinct_keys (list_t_v ls1)
     | Fail _ => F
-    | Loop => F
+    | Diverge => F
 Proof
-  Induct_on ‘ls’ >> rw [list_t_v_def] >~ [‘ListNil’] >>
-  pure_once_rewrite_tac [insert_def] >> rw []
-  >- (rw [lookup_def, lookup_raw_def, list_t_v_def])
-  >- (rw [lookup_def, lookup_raw_def, list_t_v_def]) >>
-  case_tac >> rw []
-  >- (rw [lookup_def, lookup_raw_def, list_t_v_def])
-  >- (rw [lookup_def, lookup_raw_def, list_t_v_def]) >>
-  progress
-  >- (
-    (* Disctinct keys *)
-    fs [distinct_keys_def] >>
-    rpt strip_tac >>
-    first_x_assum (qspecl_assume [‘i + 1’, ‘j + 1’]) >> fs [] >>
-    pop_assum irule >>
-    fs [index_eq, add_sub_same_eq, len_def] >>
-    int_tac) >>
-  fs [lookup_def, lookup_raw_def, list_t_v_def]
+  rw [] >>
+  qspecl_assume [‘ls’, ‘key’, ‘value’] insert_lem_aux >>
+  case_tac >> fs [] >>
+  metis_tac [distinct_keys_insert]
 QED
 
 val _ = export_theory ()
